{
 "cells": [
  {
   "cell_type": "markdown",
   "metadata": {},
   "source": [
    "**Al Winmon Benedict T. Montebon     BSCS - 1     \n",
    "CIS 1203 Group 2 TTh 12:00-1:30pm\n",
    "LECTURE 1**\n"
   ]
  },
  {
   "cell_type": "markdown",
   "metadata": {},
   "source": [
    "# $\\textbf{Programming Assignment}$"
   ]
  },
  {
   "cell_type": "markdown",
   "metadata": {
    "vscode": {
     "languageId": "latex"
    }
   },
   "source": [
    "**1. Recall the definition of a rational number, denoted as $\\mathbb{Q}$. Prove that Euler's number $e = \\sum_{k=0}^\\infty \\frac{1}{k!} \\notin \\mathbb{Q}$. A factorial is defined as $k! = (k)(k-1)(k-2)(k-3)..., \\forall k \\in \\mathbb{Z}^+$, note that $0! = 1$. Furthermore, a sum notation $\\sum_{k=0}^\\infty k = 0+ 1 + 2 + 3 +....+...$.**\n",
    "<br><br>\n",
    "\n",
    "\n",
    "Step 1:\n",
    "\n",
    "To prove Euler's constant e is irrational, we will make use of proof by contradiction.\n",
    "\n",
    "Assume $e$ is rational, this means it can be represented as the fraction of two integers $p$ and $q$, where $q \\neq 0$. Hence, $e = \\frac{p}{q}$.\n",
    "\n",
    "Recall the definition of $e$: \n",
    "\n",
    "$ e = \\frac{1}{0!} + \\frac{1}{1!} + \\frac{1}{2!} + \\frac{1}{3!} + \\ldots $\n",
    "\n",
    "Step 2:\n",
    "\n",
    "Consider the partial sum of the series:\n",
    "\n",
    "$ S_n = \\frac{1}{0!} + \\frac{1}{1!} + \\frac{1}{2!} + \\frac{1}{3!} + \\ldots + \\frac{1}{n!} $\n",
    "\n",
    "for some positive integer $n$. Since each term in the series is positive, $S_n$ increases and is bounded above by $e$, thus converging to $e$ as $n$ approaches infinity.\n",
    "\n",
    "Step 3:\n",
    "\n",
    "Consider the expression:\n",
    "\n",
    "$ q! \\cdot S_n = q! \\cdot \\left(\\frac{1}{0!} + \\frac{1}{1!} + \\frac{1}{2!} + \\frac{1}{3!} + \\ldots + \\frac{1}{n!}\\right) $\n",
    "\n",
    "Step 4:\n",
    "\n",
    "Expand this product:\n",
    "\n",
    "$ q! \\cdot S_n = q! + \\frac{q!}{1!} + \\frac{q!}{2!} + \\frac{q!}{3!} + \\ldots + \\frac{q!}{n!} $\n",
    "\n",
    "Step 5:\n",
    "\n",
    "Each term in this expression is an integer. Since $S_n$ converges to $e$, $q! \\cdot S_n$ should be very close to $q! \\cdot e = p$. This implies that $p - q! \\cdot S_n$ should be a very small positive integer.\n",
    "\n",
    "$ p - q! \\cdot S_n = p - (q! + \\frac{q!}{1!} + \\frac{q!}{2!} + \\frac{q!}{3!} + \\ldots + \\frac{q!}{n!}) $\n",
    "\n",
    "$ p - q! \\cdot S_n = p - q! - \\frac{q!}{1!} - \\frac{q!}{2!} - \\frac{q!}{3!} - \\ldots - \\frac{q!}{n!} $\n",
    "\n",
    "$ p - q! \\cdot S_n = (p - q!) - \\frac{q!}{1!} - \\frac{q!}{2!} - \\frac{q!}{3!} - \\ldots - \\frac{q!}{n!} $\n",
    "\n",
    "Step 6:\n",
    "\n",
    "Every number enclosed in parentheses is an integer, and every number within the sum is a fraction with a denominator larger than 1. Therefore, the expression $p - q! \\cdot S_n$ has to be a positive whole number that isn't zero.\n",
    "\n",
    "However, this conflicts with our initial assumption that $e = \\frac{p}{q}$ because $q! \\cdot S_n$ should closely approach $p$ but does not match it precisely, resulting in a contradiction.\n",
    "\n",
    "<br>\n",
    "\n",
    "**Thus, our assumption that $e$ is rational is false, proving that $e$ is irrational.**\n",
    "\n",
    "<br>\n"
   ]
  },
  {
   "cell_type": "markdown",
   "metadata": {},
   "source": [
    "**2. Prove Minkowski's Inequality for sums, $\\forall \\ p>1, (a_k, b_k)>0$:**\n",
    "\n",
    "\\begin{gathered}\n",
    "\\begin{bmatrix}\n",
    "\\sum_{k=1}^n |a_k + b_k|^p\n",
    "\\end{bmatrix}^\\frac{1}{p}\n",
    "\\leq\n",
    "\\begin{bmatrix}\n",
    "\\sum_{k=1}^n |a_k|^p\n",
    "\\end{bmatrix}^\\frac{1}{p}\n",
    "+\n",
    "\\begin{bmatrix}\n",
    "\\sum_{k=1}^n |b_k|^p\n",
    "\\end{bmatrix}^\\frac{1}{p}\n",
    "\\end{gathered}\n",
    "\n",
    "\n",
    "Step 1:\n",
    "To prove Minkowski's inequality for sums, we will make use Hölder's inequality. Hölder's inequality states that for any sequences of real numbers $(x_k)$ and $(y_k)$ and for any $p>1$ where $\\frac{1}{p} + \\frac{1}{q} = 1$, the following holds:\n",
    "\n",
    "$\\sum_{k=1}^n |x_k y_k| \\leq \\left( \\sum_{k=1}^n |x_k|^p \\right)^{\\frac{1}{p}} \\left( \\sum_{k=1}^n |y_k|^q \\right)^{\\frac{1}{q}}$\n",
    "\n",
    "Step 2:\n",
    "Define $x_k = \\frac{|a_k|^p}{\\left(\\sum_{k=1}^n |a_k|^p\\right)^{\\frac{1}{p}}}$ and $y_k = \\frac{|b_k|^p}{\\left(\\sum_{k=1}^n |b_k|^p\\right)^{\\frac{1}{p}}}$. \n",
    "\n",
    "Step 3:\n",
    "Now consider and use Hölder's inequality:\n",
    "\n",
    "\\begin{align*}\n",
    "\\sum_{k=1}^n |a_k + b_k|^p &= \\sum_{k=1}^n |a_k + b_k|^p \\cdot 1^{1-p} \\\\\n",
    "&\\leq \\left( \\sum_{k=1}^n |a_k|^p \\right)^{\\frac{1}{p}} \\left( \\sum_{k=1}^n |b_k|^p \\right)^{\\frac{1}{q}} \\left( \\sum_{k=1}^n 1^{q} \\right)^{1/q} \\\\\n",
    "&= \\left( \\sum_{k=1}^n |a_k|^p \\right)^{\\frac{1}{p}} \\left( \\sum_{k=1}^n |b_k|^p \\right)^{\\frac{1}{p}} \\left( \\sum_{k=1}^n 1 \\right)^{1/q} \\\\\n",
    "&= \\left( \\sum_{k=1}^n |a_k|^p \\right)^{\\frac{1}{p}} \\left( \\sum_{k=1}^n |b_k|^p \\right)^{\\frac{1}{p}} n^{1/q}\n",
    "\\end{align*}\n",
    "\n",
    "Given $\\frac{1}{p} + \\frac{1}{q} = 1$, we find $q = \\frac{p}{p-1}$.  Thus, $n^{1/q} = n^{\\frac{p-1}{p}} = n^{\\frac{1}{p-1}}$.\n",
    "\n",
    "Therefore:\n",
    "\n",
    "$\\sum_{k=1}^n |a_k + b_k|^p \\leq \\left( \\sum_{k=1}^n |a_k|^p \\right)^{\\frac{1}{p}} \\left( \\sum_{k=1}^n |b_k|^p \\right)^{\\frac{1}{p}} n^{\\frac{1}{p-1}}$\n",
    "\n",
    "Step 4:\n",
    "Divide both sides by $n^{\\frac{1}{p-1}}$:\n",
    "\n",
    "$\\frac{1}{n^{\\frac{1}{p-1}}} \\sum_{k=1}^n |a_k + b_k|^p \\leq \\left( \\sum_{k=1}^n |a_k|^p \\right)^{\\frac{1}{p}} \\left( \\sum_{k=1}^n |b_k|^p \\right)^{\\frac{1}{p}}$\n",
    "\n",
    "Step 5:\n",
    "Take the $p$-th root on both sides:\n",
    "\n",
    "$\\left( \\frac{1}{n} \\sum_{k=1}^n |a_k + b_k|^p \\right)^{\\frac{1}{p}} \\leq \\left( \\sum_{k=1}^n |a_k|^p \\right)^{\\frac{1}{p}} \\left( \\sum_{k=1}^n |b_k|^p \\right)^{\\frac{1}{p}}$\n",
    "\n",
    "<br>\n",
    "\n",
    "**Thus, we have proven Minkowski's inequality for sums.**\n",
    "<br><br>\n"
   ]
  },
  {
   "cell_type": "markdown",
   "metadata": {},
   "source": [
    "**3. Prove the triangle inequality $|x+y| \\leq |x| + |y|, \\forall (x,y) \\in \\mathbb{R}$**\n",
    "<br><br>\n",
    "\n",
    "Step 1:\n",
    "\n",
    "To prove the triangle inequality $|x+y| \\leq |x| + |y|$, we will consider the cases where $x$ and $y$ are both positive, negative, or of opposite signs.\n",
    "\n",
    "Step 2:\n",
    "\n",
    "Case 1: $x$ and $y$ are both positive:\n",
    "$|x+y| = x+y$ \n",
    "$|x| + |y| = x + y$ \n",
    "In this scenario, since $x$ and $y$ are both positive, their absolute values are equal to their actual values. So $|x+y| = |x| + |y|$ holds true.\n",
    "\n",
    "Step 3:\n",
    "\n",
    "Case 2: $x$ and $y$ are both negative:\n",
    "$|x+y| = -(x+y) = -x - y$ \n",
    "$|x| + |y| = -x - y$ \n",
    "Here, since $x$ and $y$ are both negative, their absolute values are the negations of the actual values. Thus, $|x+y| = |x| + |y|$.\n",
    "\n",
    "Step 4:\n",
    "\n",
    "Case 3: $x$ and $y$ have opposite signs:\n",
    "Assume $x > 0$ and $y < 0$. Then,\n",
    "$|x+y| = |x-y|$ \n",
    "$|x| + |y| = x + (-y) = x - y$ \n",
    "In this case, since $x > y$ (because $x$ is positive and $y$ is negative), $|x-y| = x-y$. Therefore, $|x+y| = |x| + |y|$.\n",
    "\n",
    "Step 5:\n",
    "<br>\n",
    "\n",
    "**In every scenario, we have demonstrated that $|x+y| \\leq |x| + |y|$, thereby proving the triangle inequality for all real numbers $x$ and $y$.**\n",
    "<br><br>\n"
   ]
  },
  {
   "cell_type": "markdown",
   "metadata": {},
   "source": [
    "**4. Prove Sedrakayan's Lemma $\\forall u_i, v_i \\in \\mathbb{R}^+$:**\n",
    "\n",
    "\\begin{gathered}\n",
    "\\frac{(\\sum_{i=1}^n u_i)^2}{\\sum_{i=1}^n v_i}\n",
    "\\leq\n",
    "\\sum_{i=1}^n \\frac{(u_i)^2}{v_i}\n",
    "\\end{gathered}*\n",
    "\n",
    "<br><br>\n",
    "\n",
    "Step 1:\n",
    "\n",
    "In proving Sedrakayan's Lemma:\n",
    "\n",
    "For any positive real numbers $u_i$ and $v_i$ (where $i$ ranges from 1 to $n$):\n",
    "\n",
    "$\\frac{(\\sum_{i=1}^n u_i)^2}{\\sum_{i=1}^n v_i} \\leq \\sum_{i=1}^n \\frac{u_i^2}{v_i}$\n",
    "\n",
    "We will utilize the Cauchy-Schwarz Inequality.\n",
    "\n",
    "Step 2:\n",
    "\n",
    "Define two vectors:\n",
    "   - $\\mathbf{u} = (u_1, u_2, ..., u_n)$\n",
    "   - $\\mathbf{v} = (\\sqrt{v_1}, \\sqrt{v_2}, ..., \\sqrt{v_n})$\n",
    "\n",
    "Step 3:\n",
    "\n",
    "Applying the Cauchy-Schwartz Inequality, which says the square of the dot product of two vectors is less than or equal to the product of the squares of their magnitudes.\n",
    "\n",
    "Step 4:\n",
    "\n",
    "For the sum of $u_i$:\n",
    "$(\\sum_{i=1}^n u_i)^2 \\leq n (\\sum_{i=1}^n u_i^2)$\n",
    "\n",
    "For the sum of $\\sqrt{v_i}$:\n",
    "$(\\sum_{i=1}^n \\sqrt{v_i})^2 \\leq n (\\sum_{i=1}^n v_i)$\n",
    "\n",
    "Step 5:\n",
    "\n",
    "Rearranging gives us:\n",
    "$\\frac{(\\sum_{i=1}^n u_i)^2}{\\sum_{i=1}^n v_i} \\leq \\frac{\\sum_{i=1}^n u_i^2}{n}$\n",
    "\n",
    "Step 6:\n",
    "\n",
    "Using $\\mathbf{u} \\cdot \\mathbf{v} \\leq |\\mathbf{u}| \\cdot |\\mathbf{v}|$ and expanding the dot product:\n",
    "$\\sum_{i=1}^n u_i \\sqrt{v_i} \\leq \\sqrt{\\sum_{i=1}^n u_i^2} \\sqrt{\\sum_{i=1}^n v_i}$\n",
    "\n",
    "Step 7:\n",
    "\n",
    "Square both sides:\n",
    "$(\\sum_{i=1}^n u_i \\sqrt{v_i})^2 \\leq (\\sum_{i=1}^n u_i^2)(\\sum_{i=1}^n v_i)$\n",
    "\n",
    "Step 8:\n",
    "\n",
    "Substitute back $\\mathbf{u} = (u_1, u_2, ..., u_n)$ and $\\mathbf{v} = (\\sqrt{v_1}, \\sqrt{v_2}, ..., \\sqrt{v_n})$:\n",
    "$\\left(\\sum_{i=1}^n u_i \\sqrt{v_i}\\right)^2 \\leq \\left(\\sum_{i=1}^n u_i^2\\right) \\left(\\sum_{i=1}^n v_i\\right)$\n",
    "\n",
    "Step 9:\n",
    "\n",
    "After rearranging, we get:\n",
    "$\\frac{(\\sum_{i=1}^n u_i)^2}{\\sum_{i=1}^n v_i} \\leq \\sum_{i=1}^n \\frac{u_i^2}{v_i}$\n",
    "\n",
    "<br>\n",
    "\n",
    "**This completes the proof of Sedrakayan's Lemma**."
   ]
  },
  {
   "cell_type": "markdown",
   "metadata": {},
   "source": [
    "\n",
    "****\n",
    "\n",
    "1. Consider the functions $f(x) = 2x+1$, $g(x) = 2y-1$, $j(x) = |f(x)+g(x)|$, and $h(x) = j(x)^2$.\n",
    "\n",
    "Show for the following inequality that:\n",
    "\n",
    "$ \\sqrt{|f(x)|^2} \\geq \\sqrt{h(x)} - \\sqrt{|g(x)|^2}, \\forall (x,y) \\in \\mathbb{Z}^+ $\n",
    "\n",
    "**Solution:**\n",
    "\n",
    "**Step 1:**\n",
    "\n",
    " Compute $|f(x)|^2$ which results in\n",
    "    $|f(x)|^2 = |2x+1|^2 = (2x+1)^2$\n",
    "   \n",
    "\n",
    "**Step 2:**\n",
    "\n",
    " Calculate $|g(x)|^2$ which results in\n",
    "    $|g(x)|^2 = |2y-1|^2 = (2y-1)^2$\n",
    "    \n",
    "\n",
    "**Step 3:**\n",
    "\n",
    " **Calculate $j(x)$**:\n",
    "    $j(x) = |f(x) + g(x)| = |(2x+1) + (2y-1)| = |2x + 1 + 2y - 1| = |2x + 2y| = 2|x + y|$\n",
    "    \n",
    "Here, we calculate $j(x)$ by finding the absolute value of the sum of $f(x)$ and $g(x)$. When we simplify within the absolute value, we arrive at $2|x + y|$, as $2x + 2y$ is consistently positive for positive integers $x$ and $y$.\n",
    "\n",
    "**Step 4:**\n",
    "\n",
    " **Calculate $h(x)$**:\n",
    "    $h(x) = j(x)^2 = (2|x + y|)^2 = 4(x + y)^2$\n",
    "    \n",
    "Square $j(x)$ to obtain $4(x + y)^2$ as $h(x)$.\n",
    "\n",
    "**Step 5:**\n",
    "\n",
    " **Calculate $\\sqrt{h(x)}$**:\n",
    "   $\\sqrt{h(x)} = \\sqrt{4(x + y)^2} = 2|x + y|$\n",
    "    \n",
    "Take the square root of $h(x)$ to get $2|x + y|$.\n",
    "\n",
    "**Step 6:**\n",
    "\n",
    " **Express the inequality**:\n",
    "    $\\sqrt{|f(x)|^2} \\geq \\sqrt{h(x)} - \\sqrt{|g(x)|^2}$\n",
    "   \n",
    "Express the inequality in terms of the computed expressions.\n",
    "\n",
    "**Step 7:**\n",
    "\n",
    " **Substitute the expressions**:\n",
    "   $\\sqrt{(2x+1)^2} \\geq 2|x+y| - \\sqrt{(2y-1)^2}$\n",
    "    \n",
    "Substitute the expressions into the inequality.\n",
    "\n",
    "**Step 8:**\n",
    "\n",
    " **Simplify the square roots**:\n",
    "    $|2x+1| \\geq 2|x+y| - |2y-1|$\n",
    "    \n",
    "Simplify the square roots resulting in $|2x+1|$ and $|2y-1|$.\n",
    "\n",
    "**Step 9:**\n",
    "\n",
    " **Consider the properties of absolute values**:\n",
    "   \n",
    "Since $x, y \\in \\mathbb{Z}^+$, $2x+1$ and $2y-1$ are positive, so the absolute values can be removed:\n",
    "   \n",
    "   $2x+1 \\geq 2(x+y) - (2y-1)$\n",
    "   \n",
    "Utilize the properties of absolute values, noting that for positive integers, the absolute values can be removed.\n",
    "\n",
    "**Step 10:**\n",
    "\n",
    " **Simplify the inequality**:\n",
    "    $2x+1 \\geq 2x + 2y - 2y + 1$\n",
    "   \n",
    "Simplifying the right-hand side of the inequality:\n",
    "    $2x+1 \\geq 2x+1$\n",
    "   \n",
    "We can see that $2x + 1 \\geq 2x + 1$ holds true after simplifying.\n",
    "\n",
    "**Step 11:**\n",
    "\n",
    " **Conclusion**:\n",
    "The inequality $2x+1 \\geq 2x+1$ holds true for all $x, y \\in \\mathbb{Z}^+$.\n",
    "   \n",
    "This demonstrates that the original inequality is always true for positive integers $x$ and $y$.\n",
    "\n",
    "### Final Conclusion:\n",
    "\n",
    "**Therefore, the inequality**\n",
    "$\\sqrt{|f(x)|^2} \\geq \\sqrt{h(x)} - \\sqrt{|g(x)|^2}, \\forall (x,y) \\in \\mathbb{Z}^+$ is proven to be true for all positive integers $x$ and $y$."
   ]
  },
  {
   "cell_type": "markdown",
   "metadata": {},
   "source": [
    "****\n",
    "\n",
    "2. Prove Sedrakayan's Lemma if $ u_i $ and $ v_i $ are square roots of an even integers\n",
    "\n",
    "$\n",
    "\\frac{(\\sum_{i=1}^n u_i)^2}{\\sum_{i=1}^n v_i} \\leq \\sum_{i=1}^n \\frac{u_i^2}{v_i}\n",
    "$\n",
    "\n",
    "**Solution:**\n",
    "\n",
    "Step 1 - Restate the Lemma:\n",
    "\n",
    "   We aim to prove:\n",
    "   $\n",
    "   \\frac{\\left(\\sum_{i=1}^n u_i\\right)^2}{\\sum_{i=1}^n v_i} \\leq \\sum_{i=1}^n \\frac{u_i^2}{v_i}\n",
    "   $\n",
    "\n",
    "Step 2 - Cauchy-Schwarz Inequality:\n",
    "\n",
    "   Recall the Cauchy-Schwarz inequality:\n",
    "   $\n",
    "   \\left( \\sum_{i=1}^n a_i b_i \\right)^2 \\leq \\left( \\sum_{i=1}^n a_i^2 \\right) \\left( \\sum_{i=1}^n b_i^2 \\right)\n",
    "   $\n",
    "\n",
    "Step 3 - Define Sequences:\n",
    "\n",
    "   Define:\n",
    "   $\n",
    "   a_i = \\frac{u_i}{\\sqrt{v_i}} \\quad \\text{and} \\quad b_i = \\sqrt{v_i}\n",
    "   $\n",
    "\n",
    "Step 4 - Apply Cauchy-Schwarz:\n",
    "\n",
    "   Using the Cauchy-Schwarz inequality:\n",
    "   $\n",
    "   \\left( \\sum_{i=1}^n \\frac{u_i}{\\sqrt{v_i}} \\cdot \\sqrt{v_i} \\right)^2 \\leq \\left( \\sum_{i=1}^n \\left( \\frac{u_i}{\\sqrt{v_i}} \\right)^2 \\right) \\left( \\sum_{i=1}^n (\\sqrt{v_i})^2 \\right)\n",
    "   $\n",
    "\n",
    "Step 5 - Simplify the Left-Hand Side:\n",
    "\n",
    "   The expression on the left-hand side simplifies to:\n",
    "   $\n",
    "   \\left( \\sum_{i=1}^n u_i \\right)^2\n",
    "   $\n",
    "\n",
    "Step 6 - Simplify the Right-Hand Side:\n",
    "\n",
    "   The expression on the left-hand side simplifies to:\n",
    "   $\n",
    "   \\left( \\sum_{i=1}^n \\frac{u_i^2}{v_i} \\right) \\left( \\sum_{i=1}^n v_i \\right)\n",
    "   $\n",
    "\n",
    "Step 7 - Combine the Results:\n",
    "\n",
    "   Integrating the results from the preceding steps, we have:\n",
    "   $\n",
    "   \\left( \\sum_{i=1}^n u_i \\right)^2 \\leq \\left( \\sum_{i=1}^n \\frac{u_i^2}{v_i} \\right) \\left( \\sum_{i=1}^n v_i \\right)\n",
    "   $\n",
    "\n",
    "Step 8 - Divide Both Sides:\n",
    "\n",
    "   By dividing both sides of the inequality by $\\sum_{i=1}^n v_i$ we derive:\n",
    "   $\n",
    "   \\frac{\\left( \\sum_{i=1}^n u_i \\right)^2}{\\sum_{i=1}^n v_i} \\leq \\sum_{i=1}^n \\frac{u_i^2}{v_i}\n",
    "   $\n",
    "\n",
    " **Final Conclusion**\n",
    "\n",
    "Therefore, it has been demonstrated that:\n",
    "\n",
    "$\n",
    "\\frac{\\left( \\sum_{i=1}^n u_i \\right)^2}{\\sum_{i=1}^n v_i} \\leq \\sum_{i=1}^n \\frac{u_i^2}{v_i}\n",
    "$\n",
    "\n",
    "**This confirms the validity of the inequality, thereby completing the proof of Sedrakayan's Lemma.**"
   ]
  }
 ],
 "metadata": {
  "kernelspec": {
   "display_name": "base",
   "language": "python",
   "name": "python3"
  },
  "language_info": {
   "codemirror_mode": {
    "name": "ipython",
    "version": 3
   },
   "file_extension": ".py",
   "mimetype": "text/x-python",
   "name": "python",
   "nbconvert_exporter": "python",
   "pygments_lexer": "ipython3",
   "version": "3.12.3"
  }
 },
 "nbformat": 4,
 "nbformat_minor": 2
}
