{
 "cells": [
  {
   "cell_type": "markdown",
   "metadata": {},
   "source": [
    "**Al Winmon Benedict T. Montebon     BSCS - 1     \n",
    "CIS 1203 Group 2 TTh 12:00-1:30pm\n",
    "LECTURE 2**\n"
   ]
  },
  {
   "cell_type": "markdown",
   "metadata": {},
   "source": [
    "# $\\textbf{Programming Assignment}$"
   ]
  },
  {
   "cell_type": "markdown",
   "metadata": {},
   "source": [
    "\n",
    "**Task 1:\n",
    "Consider the following experiment:**\n",
    "1. The experiment consists of $n$ identical trials.\n",
    "2. The outcome of each trial falls into one of $k$ classes or cells.\n",
    "3. The probability that the outcome of a single trial falls into cell $i$ is $p_i$, where $i = 1, 2, ..., k$, and remains the same from trial to trial. Note that $\\sum_{i=1}^k p_i = 1$.\n",
    "4. The trials are independent.\n",
    "5. The random variables of interest are $Y_1, Y_2, ..., Y_k$, where $Y_i$ equals the number of trials for which the outcome falls into cell $i$. Note that $\\sum_{i=1}^k Y_i = n$.\n",
    "6. The joint probability distribution $P(y) = \\frac{n!}{y_1!y_2!y_3!...y_n!} P_1^{y_1} P_2^{y_2} P_3^{y_3}....P_n^{y_n}$\n",
    "\n",
    "\n",
    "**Question 1: Show that the expected value $E[y] = \\Sigma y \\cdot P(y) = n \\cdot p_i$**\n",
    "\n",
    "Step 1:\n",
    "The expected value of a random variable $Y_i$ can be calculated using the formula $E[Y_i] = \\sum_{y} y \\cdot P(y)$\n",
    "\n",
    "Step 2:\n",
    "Using the given joint probability distribution, we can determine $E[Y_i]$ as follows:\n",
    "$E[Y_i] = \\sum_{y} y \\cdot P(y) = \\sum_{y} y \\cdot \\frac{n!}{y_1!y_2!y_3!\\cdots y_n!} P_1^{y_1} P_2^{y_2} P_3^{y_3}\\cdots P_n^{y_n}$\n",
    "\n",
    "Step 3:\n",
    "Note that $Y_i$ represents the number of trials where the outcome falls into cell $i$.\n",
    "\n",
    "Step 4:\n",
    "It follows that $Y_i$ equals to $n \\cdot p_i$, where $p_i$ denotes the probability of the outcome falling into cell $i$ in a single trial.\n",
    "\n",
    "Step 5:\n",
    "Thus, we have $E[Y_i] = n \\cdot p_i$. **QED**\n",
    "\n",
    "**Question 2: Given the following data**\n",
    "\n",
    "\\begin{array}{|c|c|}\n",
    "\\hline\n",
    "\\text{Age} & \\text{Proportion} \\\\\n",
    "\\hline\n",
    "18-24 & 0.18 \\\\\n",
    "25-34 & 0.23 \\\\\n",
    "35-44 & 0.16 \\\\\n",
    "45-64 & 0.27 \\\\\n",
    "65-100 & 0.16 \\\\\n",
    "\\hline\n",
    "\\end{array}\n",
    "\n",
    "*If 500 adults are randomly sampled, determine the probability that the sample includes 100 individuals aged 18-24, 200 aged 25-34, and 200 aged 45-64. What is the anticipated value to obtain a person aged 65 and above?*\n",
    "\n",
    "Step 1:\n",
    "To calculate the probability of the sample containing a specific number of individuals in each age group, we use the multinomial distribution formula:\n",
    "\n",
    "$P(y_1, y_2, y_3, y_4, y_5) = \\frac{500!}{100! \\cdot 200! \\cdot 200! \\cdot 0! \\cdot 0!} \\times 0.18^{100} \\times 0.23^{200} \\times 0.16^{200} \\times 0.27^0 \\times 0.16^0$\n",
    "\n",
    "Step 2:\n",
    "Where:\n",
    "- $y_1 = 100$ (individuals aged 18-24)\n",
    "- $y_2 = 200$ (individuals aged 25-34)\n",
    "- $y_3 = 200$ (individuals aged 35-44)\n",
    "- $y_4 = 0$ (individuals aged 45-64)\n",
    "- $y_5 = 0$ (individuals aged 65-100)\n",
    "\n",
    "Subsequent to computing this probability, we can ascertain the expected value to obtain a person aged 65 and above by summing up the products of the probability of each age group and the count of individuals in that age group.\n",
    "\n",
    "Step 3:\n",
    "Let $p_{65+}$ represent the probability of an individual being aged 65 and above.\n",
    "\n",
    "Step 4:\n",
    "Given the probabilities of all other age groups, we are able to find $p_{65+}$ by subtracting the sum of probabilities of other age groups from 1.\n",
    "$p_{65+} = 1 - (0.18 + 0.23 + 0.16 + 0.27) = 0.16$\n",
    "\n",
    "Step 5:\n",
    "To find the expected number of individuals aged 65 and above in a sample of 500 adults, we multiply the probability $p_{65+}$ by the total sample size:\n",
    "$\\text{Expected count of individuals aged 65 and above} = 500 \\times 0.16 = 80$\n",
    "\n",
    "Step 6:\n",
    "Therefore, the expected number of individuals aged 65 and above in the sample is **80**.\n",
    "\n"
   ]
  },
  {
   "cell_type": "markdown",
   "metadata": {},
   "source": [
    "Task 2: Consider the following experiment:\n",
    "1. The experiment consists of a fixed number, $n$, of identical trials.\n",
    "2. Each trial results in one of two outcomes: success, $S$, or failure, $F$.\n",
    "3. The probability of success on a single trial is equal to some value $p$ and remains the same from trial to trial. The probability of a failure is equal to $q = (1 - p)$.\n",
    "4. The trials are independent.\n",
    "5. The random variable of interest is $Y$, the number of successes observed during the $n$ trials.\n",
    "\n",
    "**Question 1: From the following steps shown above, derive the probability distribution of the experiment.\n",
    "To derive the probability distribution of the experiment described in the steps provided, we need to find the probability mass function (PMF) for the random variable $Y$, which represents the number of successes observed during the $n$ trials.**\n",
    "\n",
    "\n",
    "Step 1:\n",
    "Define $ Y=y $ as the event of observing exactly $ y $ successes out of $ n $ trials.\n",
    "\n",
    "Step 2:\n",
    "The probability of observing exactly $ y $ successes and $ (n - y) $ failures is given by the binomial probability formula:\n",
    "$$ P(Y = y) = \\binom{n}{y} \\times p^y \\times (1 - p)^{n - y} $$\n",
    "\n",
    "Step 3:\n",
    "Let:\n",
    "- $ n $ be the fixed number of trial,\n",
    "- $ p $ be the probability of success on each trial,\n",
    "- $ \\binom{n}{y} $ be the number of combinations for choosing $ y $ successes out of $ n $ trials (combinations), and\n",
    "- $ (1 - p)^{n - y} $ be the probability of encountering $ (n - y) $ failures.\n",
    "\n",
    "Therfore, the probability distribution of $ Y $ can be expressed as:\n",
    "$$ P(Y = y) = \\binom{n}{y} \\times p^y \\times (1 - p)^{n - y} $$\n",
    "where $ y $ ranges from 0 to $ n $.\n",
    "\n",
    "Step 4:\n",
    "This probability distribution describes the likelihood of each possible number of successes in the $ n $ trials.\n"
   ]
  },
  {
   "cell_type": "markdown",
   "metadata": {},
   "source": [
    "\n",
    "\n",
    "**Question 2: Show that the expectation of this probability distribution is $E[y] = \\Sigma y \\cdot P(y) = np$.**\n",
    "To answer Question 2, let's first understand the expectation of a probability distribution.\n",
    "\n",
    "\n",
    "Step 1:\n",
    "The expected value, denoted as $E[y]$, represents the average value of the random variable $Y$ over many trials. Mathematically, it's calculated as the sum of each possible outcome $y$ multiplied by its probability $P(y)$.\n",
    "\n",
    "Step 2:\n",
    "In this context, $Y$ symbolizes the count of successes observed in $n$ trials, where the likelihood of success in each trial is $p$. The probability distribution of $Y$ adheres to a binomial distribution.\n",
    "\n",
    "The probability mass function (PMF) of a binomial distribution is expressed as:\n",
    "$ P(y) = \\binom{n}{y} p^y (1 - p)^{n - y} $\n",
    "where $\\binom{n}{y}$ represents the binomial coefficient.\n",
    "\n",
    "Step 3:\n",
    "To find the expectation $E[y]$, we sum over all possible values of $y$ multiplied by their respective probabilities:\n",
    "$ E[y] = \\sum_{y=0}^{n} y \\cdot P(y) $\n",
    "\n",
    "Step 4:\n",
    "By substituting the PMF of the binomial distribution, the expression becomes:\n",
    "$ E[y] = \\sum_{y=0}^{n} y \\cdot \\binom{n}{y} p^y (1 - p)^{n - y} $\n",
    "\n",
    "Step 5:\n",
    "Using properties of the binomial coefficient and the linearity of expectation, we can simplify this expression to:\n",
    "$ E[y] = \\sum_{y=1}^{n} y \\cdot \\binom{n}{y} p^y (1 - p)^{n - y} $\n",
    "\n",
    "$ = \\sum_{y=1}^{n} \\frac{n!}{(y-1)!(n-y)!} p^y (1 - p)^{n - y} $\n",
    "\n",
    "$ = \\sum_{y=1}^{n} np \\sum_{y=1}^{n} \\binom{n-1}{y-1} p^{y-1} (1 - p)^{(n-1) - (y-1)} $\n",
    "\n",
    "$ = np \\sum_{k=0}^{n-1} \\binom{n-1}{k} p^k (1 - p)^{(n-1) - k} $\n",
    "\n",
    "$ = np \\cdot 1 $\n",
    "\n",
    "$ = np $\n",
    "\n",
    "Step 6:\n",
    "Thus, the expected value of this probability distribution is $E[y] = np$.\n",
    "\n",
    "**Question 3: Experience has shown that 30% of all persons afflicted by a certain illness recover. A drug company has developed a new medication. Ten people with the illness were selected at random and received the medication; nine recovered shortly thereafter. Suppose that the medication was absolutely worthless. What is the probability that at least nine of ten receiving the medication will recover?**\n",
    "\n",
    "To find the final answer, we first calculate the probabilities $P(Y = 9)$ and $P(Y = 10)$, then sum them up to get $P(Y \\geq 9)$.\n",
    "\n",
    "Step 1:\n",
    "\n",
    "For $k = 9$:\n",
    "\n",
    "$P(Y = 9) = \\binom{10}{9} \\times (0.30)^9 \\times (0.70)^1$\n",
    "\n",
    "$P(Y = 9) = 10 \\times (0.30)^9 \\times (0.70)^1$\n",
    "\n",
    "$P(Y = 9) \\approx 0.121$\n",
    "\n",
    "Step 2:\n",
    "\n",
    "For $k = 10$:\n",
    "\n",
    "$P(Y = 10) = \\binom{10}{10} \\times (0.30)^{10} \\times (0.70)^0$\n",
    "\n",
    "$P(Y = 10) = (0.30)^{10} \\times 1$\n",
    "\n",
    "$P(Y = 10) \\approx 0.028$\n",
    "\n",
    "Step 3:\n",
    "\n",
    "Summing these probabilities yields $P(Y \\geq 9)$:\n",
    "\n",
    "$P(Y \\geq 9) = P(Y = 9) + P(Y = 10)$\n",
    "\n",
    "$P(Y \\geq 9) \\approx 0.121 + 0.028$\n",
    "\n",
    "$P(Y \\geq 9) \\approx 0.149$\n",
    "\n",
    "Step 4:\n",
    "\n",
    "So, the probability that at least nine out of ten recipients will recover is approximately $0.149$, or $14.9\\%$.\n",
    "\n",
    "\n",
    "**Question 4: Suppose that a lot of 5000 electrical fuses contains 5% defectives. If a sample of 5 fuses is tested, find the probability of observing at least one defective.**\n",
    "\n",
    "\n",
    "To find the probability of observing at least one defective fuse in a sample of 5 from a lot of 5000 electrical fuses containing 5% defectives, we can use the concept of binomial probability.\n",
    "\n",
    "Step 1:\n",
    "Let $Y$ denote the count of defective fuses observed during the 5 trials.\n",
    "\n",
    "We aim to calculate $P(Y \\geq 1)$, representing the probability of observing at least one defective fuse.\n",
    "\n",
    "Step 2:\n",
    "By applying the complement rule, we can find this probability as:\n",
    "$ P(Y \\geq 1) = 1 - P(Y = 0) $\n",
    "\n",
    "Step 3:\n",
    "To determine $P(Y = 0)$ (the probability of observing no defective fuses), we employ the binomial probability formula:\n",
    "\n",
    "$ P(Y = k) = \\binom{n}{k} \\times p^k \\times q^{n-k} $\n",
    "\n",
    "Step 4:\n",
    "Here $\\binom{n}{k}$ represents the number of combinations of choosing $k$ successes out of $n$ trials.\n",
    "\n",
    "Step 5:\n",
    "In this case, $k = 0$ (no defective fuses), $n = 5$, $p = 0.05$, and $q = 0.95$.\n",
    "\n",
    "Step 6:\n",
    "Calculating $P(Y \\geq 1)$ yields:\n",
    "\n",
    "$ P(Y \\geq 1) = 1 - P(Y = 0) $\n",
    "\n",
    "$ = 1 - \\binom{5}{0} \\times 0.05^0 \\times 0.95^5 $\n",
    "\n",
    "$ = 1 - 1 \\times 1 \\times (0.95)^5 $\n",
    "\n",
    "$ = 1 - 1 \\times 1 \\times 0.7737809375$\n",
    "\n",
    "$ \\approx 1 - 0.7737809375 $\n",
    "\n",
    "$ \\approx 0.2262190625 $\n",
    "\n",
    "Step 7:\n",
    "Thus, the probability of observing at least one defective fuse in a sample of 5 is approximately $0.2262$, or $22.62\\%$.\n",
    "\n",
    "\n",
    "**Task 3: Consider a probability distribution of $p(y) = \\frac{\\lambda^y}{y!} e^{-\\lambda}$.**\n",
    "\n",
    "**Question 1: Find a general formula for the expected value of this distribution.**\n",
    "\n",
    "\n",
    "Step 1:\n",
    "To find the expected value of this Poisson distribution with parameter $\\lambda$, denoted as $E(Y)$, we apply the definition of expected value for discrete random variables:\n",
    "\n",
    "$ E(Y) = \\sum_{y=0}^{\\infty} y \\cdot p(y) $\n",
    "\n",
    "Step 2:\n",
    "By substituting the provided expression for $p(y)$ into the equation, we obtain:\n",
    "\n",
    "$ E(Y) = \\sum_{y=0}^{\\infty} y \\cdot \\frac{\\lambda^y}{y!} e^{-\\lambda} $\n",
    "\n",
    "Step 3:\n",
    "To solve this, we leverage the principle that the total sum of probabilities in a probability distribution equals $1$. Thus, we rewrite the sum as follows:\n",
    "\n",
    "$ E(Y) = \\sum_{y=1}^{\\infty} y \\cdot p(y) + 0 \\cdot \\frac{\\lambda^0}{0!} e^{-\\lambda} $\n",
    "\n",
    "Step 4:\n",
    "Now, we simplify the terms where $y$ is greater than $0$:\n",
    "\n",
    "$ E(Y) = \\sum_{y=1}^{\\infty} y \\cdot p(y) $\n",
    "\n",
    "\n",
    "Step 5:\n",
    "For further simplification, we extract $e^{-\\lambda}$ outside the summation:\n",
    "\n",
    "$ E(Y) = e^{-\\lambda} \\sum_{y=1}^{\\infty} \\frac{\\lambda^y}{(y-1)!} $\n",
    "\n",
    "Step 6:\n",
    "Now, let's make a substitution to simplify the expression inside the sum. Let $k = y - 1$, then $y = k + 1$. Also, when $y = 1$, $k = 0$, and as $y$ approaches infinity, $k$ also approaches infinity. With these substitutions, the sum becomes:\n",
    "\n",
    "$ E(Y) = e^{-\\lambda} \\sum_{k=0}^{\\infty} \\frac{\\lambda^{k+1}}{k!} $\n",
    "\n",
    "$ E(Y) = e^{-\\lambda} \\lambda \\sum_{k=0}^{\\infty} \\frac{\\lambda^k}{k!} $\n",
    "\n",
    "Step 7:\n",
    "Recognizing that the sum inside the expression represents the Taylor series expansion of $e^\\lambda$, which is $e^\\lambda$, we conclude:\n",
    "\n",
    "$ E(Y) = e^{-\\lambda} \\lambda e^\\lambda $\n",
    "\n",
    "$ E(Y) = \\lambda $\n",
    "\n",
    "Step 8:\n",
    "Therefore, the general formula for the expected value of the given distribution is simply $\\lambda$.\n"
   ]
  },
  {
   "cell_type": "markdown",
   "metadata": {},
   "source": [
    "\n",
    "**Question 2: A certain type of tree has seedlings randomly dispersed in a large area, with the mean density of seedlings being approximately five per square yard. If a forester randomly locates ten 1-square-yard sampling regions in the area, find the probability that none of the regions will contain seedlings.**\n",
    "\n",
    "\n",
    "Step 1:\n",
    "Here, we're looking at a Poisson distribution, which is represented by the formula:\n",
    "\n",
    "$ p(y) = \\frac{\\lambda^y}{y!} e^{-\\lambda} $\n",
    "\n",
    "Step 2:\n",
    "In this formula:\n",
    "- $\\lambda$ stands for the average rate, indicating the mean density of seedlings per square yard.\n",
    "- $y$ represents the count of seedlings within a specific region.\n",
    "\n",
    "Step 3:\n",
    "Given that the mean density of seedlings is five per square yard, we have $\\lambda = 5$.\n",
    "\n",
    "Step 4:\n",
    "Our aim is to determine the likelihood of finding no seedlings in any region. This translates to the probability of having $y = 0$ seedlings in a region. Substituting $\\lambda = 5$ and $y = 0$ into the Poisson distribution formula gives us:\n",
    "\n",
    "$ p(0) = \\frac{5^0}{0!} e^{-5} = e^{-5} $\n",
    "\n",
    "Step 5:\n",
    "We can calculate this probability:\n",
    "\n",
    "$ p(0) \\approx e^{-5} \\approx 0.00674 $\n",
    "\n",
    "Step 6:\n",
    "Therefore, the probability of encountering no seedlings in any region is approximately $0.00674$, or $0.674\\%$."
   ]
  }
 ],
 "metadata": {
  "kernelspec": {
   "display_name": "base",
   "language": "python",
   "name": "python3"
  },
  "language_info": {
   "codemirror_mode": {
    "name": "ipython",
    "version": 3
   },
   "file_extension": ".py",
   "mimetype": "text/x-python",
   "name": "python",
   "nbconvert_exporter": "python",
   "pygments_lexer": "ipython3",
   "version": "3.11.7"
  }
 },
 "nbformat": 4,
 "nbformat_minor": 2
}
